vera/VerilogSemantics.v
@@ -152,6 +152,7 @@ Module CombinationalOnly.
     eval_binop Verilog.BinaryStar l r := bv_binop (@BV.bv_mult _) l r;
     eval_binop Verilog.BinaryBitwiseAnd l r := bitwise_binop and_bit l r;
     eval_binop Verilog.BinaryBitwiseOr l r := bitwise_binop or_bit l r;
+    eval_binop Verilog.BinaryShiftLeft l r := _;
     eval_binop op l r := _
   .
   Admit Obligations.
